

HW1

1) a) $\langle x | \hat{x} | x' \rangle = x \delta(x-x')$

$\langle k | \hat{x} | k' \rangle = i\hbar^2/2p \delta(p-p')$

This is from Fourier transform of $p = -i\hbar^2/2x$

b) $\langle x | \hat{p} | x' \rangle = -i\hbar^2/2x \delta(x-x')$

$\langle k | \hat{p} | k' \rangle = k \delta(k-k')$

c) $\langle x | \hat{p}_{kin} | x' \rangle = \langle x | \frac{k^2}{2m} | x' \rangle \rightarrow \frac{1}{2m} (-i\hbar^2/2x)^2 \delta(x-x')$

$\langle k | \hat{p}_{kin} | k' \rangle = \langle k | \frac{k^2}{2m} | k' \rangle \rightarrow \frac{p^2}{2m} \delta(k-k')$

d) $\langle x | \hat{V} | x' \rangle \rightarrow \langle x | \hat{V}(x) | x' \rangle \rightarrow V(x) \delta(x-x')$

$\langle k | \hat{V} | k' \rangle \rightarrow \langle k | \hat{V}(x) | k' \rangle \rightarrow V(i\hbar^2/2p) \delta(k-k')$

e) $L = \hat{x} \times \hat{k} \rightarrow \begin{vmatrix} \hat{x} & \hat{y} & \hat{z} \\ x & y & z \\ k_x & k_y & k_z \end{vmatrix}$

$L_x = yk_z - zk_y \quad L_y = xk_z - zk_x \quad L_z = xk_y - yk_x$

$\langle x | \hat{L} | x' \rangle \rightarrow L_x = -i\hbar (y^2/2z - z^2/2y) \delta(x-x')$

$L_y = -i\hbar (x^2/2z - z^2/2x) \delta(x-x')$

$L_z = i\hbar (x^2/2y - y^2/2x) \delta(x-x')$

$\langle k | \hat{L} | k' \rangle \rightarrow L_x = i\hbar (k_z^2/2k_y - k_y^2/2k_z) \delta(k-k')$

$L_y = i\hbar (k_z^2/2k_x - k_x^2/2k_z) \delta(k-k')$

$L_z = i\hbar (k_y^2/2k_x - k_x^2/2k_y) \delta(k-k')$

Both delta function and partial derivative b/c function of both \hat{x}/\hat{k}

$$f) \hat{V} = \frac{d\hat{k}}{dt} \rightarrow \frac{i}{\hbar} [\hat{H}, \hat{x}] \rightarrow \frac{i}{\hbar} \left[\frac{\hat{k}^2}{2m} + \hat{V}(x), \hat{x} \right]$$

$$[\hat{V}(x), \hat{x}] = 0$$

a general formula is $\frac{d\hat{A}}{dt} = \frac{i}{\hbar} [\hat{H}, \hat{A}]$ Heisenberg eqn of motion

$$= \frac{i}{\hbar} \left[\frac{\hat{k}^2}{2m}, \hat{x} \right] = \frac{i}{\hbar} \frac{1}{2m} [\hat{k}^2, \hat{x}] \quad [\hat{k}^2, \hat{x}] = \hat{k}[\hat{k}, \hat{x}] + [\hat{k}, \hat{x}]\hat{k}$$

not sure if you're expecting me to show how this is true, I just looked up the properties for it

$$[\hat{x}, \hat{k}] = i\hbar \rightarrow [\hat{k}, \hat{x}] = -i\hbar \quad [\hat{k}^2, \hat{x}] = \hat{k}i\hbar - i\hbar\hat{k} = -2i\hbar\hat{k}$$

$$= \frac{i}{\hbar} \frac{1}{2m} (-2i\hbar\hat{k}) \quad i^2 \rightarrow -1$$

$\hat{V} = \frac{\hat{k}}{m}$, so it is momentum over mass I guess...

$$\langle x | \hat{V} | x' \rangle \rightarrow \langle x | \frac{\hat{k}}{m} | x' \rangle = -i\hbar/m^2 \delta(x-x')$$

$$\langle k | \hat{V} | k' \rangle \rightarrow \langle k | \frac{\hat{k}}{m} | k' \rangle = \frac{k}{m} \delta(k-k')$$

2) a) (3D) $g_{dim}(E) = \lim_{E \rightarrow 0} \frac{\# \text{ states within } [E, E+dE]}{dE \cdot \text{Volume}} \left[\frac{1}{dV \cdot m^{dim}} \right]$

Set numerator to integral/V

$$\Delta^{dim} k = \frac{(2\pi)^{dim}}{V} \int_{E_k}^{E_k+dE} d^3k$$

$$= \frac{4\pi}{(2\pi)^3} \int_{E_k}^{E_k+dE} k^2 dk \cdot \frac{1}{dE}$$

$$\int_{E_k}^{E_k+dE} d^3k = \frac{(2\pi)^3}{(2\pi)^3} \int_{E_k}^{E_k+dE} d^3k = \frac{\int_{E_k}^{E_k+dE} d^3k}{(2\pi)^3} \cdot \frac{1}{dE}$$

Cartesian \rightarrow spherical

$$d^3k = dk_x dk_y dk_z = k^2 \sin\theta dk d\theta d\phi$$

convert back to limit

$$= \lim_{E \rightarrow 0} \frac{4\pi}{(2\pi)^3} k^2(E) \frac{dk}{dE}$$

$$= \lim_{E \rightarrow 0} \frac{4\pi}{(2\pi)^3} k^2(E) \frac{m}{\hbar^2 k} = \frac{4\pi}{(2\pi)^3} \frac{km}{\hbar^2}$$

$$= \frac{4\pi}{8\pi^2} \frac{m}{\hbar^2} \sqrt{\frac{2mE}{\hbar^2}} = \left[\frac{1}{4\pi^2} \left(\frac{2m}{\hbar^2} \right)^{1/2} \sqrt{E} \right]$$

$$E = \frac{\hbar^2 k^2}{2m} \quad dE = \frac{\hbar^2 k}{m} dk$$

$$dE = \frac{\hbar^2 k}{m} dk$$

$$dE/dk = \frac{\hbar^2 k}{m} \quad \frac{dk}{dE} = \frac{m}{\hbar^2 k}$$

$$k = \sqrt{\frac{2mE}{\hbar^2}}$$

$$b) \textcircled{20} \lim_{\Delta \epsilon \rightarrow 0} \frac{\# \text{ states}}{\Delta \epsilon \cdot V} = \frac{\int_{\epsilon_k}^{\epsilon_k + \Delta \epsilon} d^2 k \cdot \frac{1}{\Delta \epsilon \cdot SA}}{(2\pi)^2}$$

$$d^2 k = dk_x dk_y \rightarrow \text{Polar}$$

$$k dk d\phi = \frac{2\pi}{(2\pi)^2} \int_{\epsilon_k}^{\epsilon_k + \Delta \epsilon} \frac{1}{(2\pi)^2} \int_0^{2\pi} k dk d\phi \cdot \frac{1}{\Delta \epsilon}$$

$$= \frac{2\pi}{(2\pi)^2} \int_{\epsilon_k}^{\epsilon_k + \Delta \epsilon} k dk \cdot \frac{1}{\Delta \epsilon}$$

back to limit

$$\lim_{\Delta \epsilon \rightarrow 0} \frac{1}{2\pi} k(\epsilon) \frac{dk}{d\epsilon} = \frac{1}{2\pi} k \frac{m}{\hbar^2 k} = \frac{1}{2\pi} \frac{m}{\hbar^2}$$

$$dk/d\epsilon = \frac{m}{\hbar^2 k}$$

$$c) \textcircled{10} \int_{\epsilon_k}^{\epsilon_k + \Delta \epsilon} \frac{dk}{2\pi} \cdot \frac{1}{\Delta \epsilon \cdot k} \rightarrow \frac{1}{2\pi} \int_{\epsilon_k}^{\epsilon_k + \Delta \epsilon} \frac{dk}{k} = \frac{1}{\Delta \epsilon} \frac{m}{\hbar^2 k}$$

$$= \frac{1}{\Delta \epsilon} \frac{dk}{k} = \frac{1}{\Delta \epsilon} \frac{m}{\hbar^2 k}$$

$$= \frac{m}{\hbar^2 k} \quad k = \sqrt{\frac{2m\epsilon}{\hbar^2}}$$

$$= \frac{m}{\hbar^2} \sqrt{\frac{\hbar^2}{2m\epsilon}} = \frac{1}{\hbar} \left(\frac{m}{2\epsilon} \right)$$

$$d) \text{ dim } > 3 \quad g_{\text{dim}}(\epsilon) = \lim_{\Delta \epsilon \rightarrow 0} \frac{\# \text{ states within } [\epsilon, \epsilon + \Delta \epsilon]}{\Delta \epsilon \cdot \text{Vol}_{\text{dim}}}$$

$$g_{\text{dim}}(\epsilon) = \frac{\int_{\epsilon_k}^{\epsilon_k + \Delta \epsilon} d^{\text{dim}} k \cdot \frac{1}{\Delta \epsilon \cdot \text{Vol}_{\text{dim}}}}{(2\pi)^{\text{dim}}}$$

$$d^{\text{dim}} k \rightarrow r^{\text{dim}-1} \left(\frac{2\pi n_b}{\Gamma(n_b)} \right)$$

formula for total solid angle in \uparrow space

$$\frac{1}{(2\pi)^{\text{dim}}} \left(\frac{2\pi^{\text{dim}/2}}{\Gamma(\text{dim}/2)} \right) \int_{\epsilon_k}^{\epsilon_k + \Delta \epsilon} k^{\text{dim}} \cdot \frac{1}{\Delta \epsilon}$$

$$= \lim_{\Delta \epsilon \rightarrow 0} \frac{1}{(2\pi)^{\text{dim}}} \left(\frac{2\pi^{\text{dim}/2}}{\Gamma(\text{dim}/2)} \right) k^{\text{dim}}(\epsilon) \frac{dk}{d\epsilon} \Big|_{\epsilon}$$

$$= \frac{1}{(2\pi)^{\text{dim}}} \left(\frac{2\pi^{\text{dim}/2}}{\Gamma(\text{dim}/2)} \right) \left(\frac{2m\epsilon}{\hbar^2} \right)^{\frac{\text{dim}-1}{2}} \frac{m}{\hbar^2} \rightarrow \frac{1}{(2\pi)^{\text{dim}}} \left(\frac{2\pi^{\text{dim}/2}}{\Gamma(\text{dim}/2)} \right) \left(\frac{2m^2 \epsilon}{\hbar^4} \right)^{\frac{\text{dim}-1}{2}}$$

e) (C0) $g_{\text{co}}(\epsilon) = \sum_n \delta(\epsilon - \epsilon_n)$

$$g_{\text{dim}}(\epsilon) = \frac{\int d^{\text{dim}} k \cdot \frac{1}{\partial \epsilon \cdot V_{\text{dim}}} \rightarrow \frac{1}{(2\pi)^{\text{dim}}} \int d^{\text{dim}} k \cdot 1 / \partial \epsilon \rightarrow \frac{1}{(2\pi)^{\text{dim}}} \int d^{\text{dim}} k \delta(\epsilon - \epsilon_k)$$

$$\frac{1}{(2\pi)^{\text{dim}}} \int d^{\text{dim}} k \delta(\epsilon - \epsilon_k) \rightarrow \left(\frac{1}{(2\pi)^{\text{dim}}} \sum_n \delta(\epsilon - \epsilon_n) \right), \text{ or call it } \left(\frac{1}{V_{\text{dim}}} \sum_n \delta(\epsilon - \epsilon_n) \right)$$

for (0D), $(2\pi)^0 \rightarrow 1$, so $g_{\text{co}} = \sum_n \delta(\epsilon - \epsilon_n)$

3) $E_{\text{r, int}} = \frac{\hbar^2 \omega^2}{2m} n^2 + \frac{\hbar^2 k^2}{2m}$ $m = .067 m_0$ $m_0 = 9.1 \times 10^{-31} \text{ kg}$